commit

AP/Inference/Basic.lean
@@ -2,148 +2,126 @@ import AP.Util
 
 namespace Inference
 
-inductive Expr where
-| var : ℕ → Expr
-| not : Expr → Expr
-| imp : Expr → Expr → Expr
+inductive Stat where
+| var : ℕ → Stat
+| not : Stat → Stat
+| imp : Stat → Stat → Stat
+deriving Inhabited, DecidableEq
 
-inductive Proof' : Expr → Type where
-| ax₁ : ∀ (P Q : Expr), Proof' # .imp P # .imp Q P
-| ax₂ : ∀ (P Q R : Expr), Proof' # .imp
-  (.imp P # .imp Q R) # .imp (.imp P Q) # .imp P R
-| ax₃ : ∀ (P Q : Expr), Proof' # .imp
-  (.imp (.not P) (.not Q)) # .imp Q P
-| mp : ∀ {P Q}, Proof' (.imp P Q) → Proof' P → Proof' Q
+inductive Proof' : Type where
+| ax₁ : Stat → Stat → Proof'
+| ax₂ : Stat → Stat → Stat → Proof'
+| ax₃ : Stat → Stat → Proof'
+| mp : Proof' → Proof' → Proof'
+deriving Inhabited, DecidableEq
 
-inductive Proof (e : Expr) : Prop where
-| mk : Proof' e → Proof e
+@[simp]
+def Proof'.stat (p : Proof') : Option Stat :=
+  match p with
+  | .ax₁ P Q => some # .imp P # .imp Q P
+  | .ax₂ P Q R => some # .imp
+    (.imp P # .imp Q R) # .imp (.imp P Q) # .imp P R
+  | .ax₃ P Q => some # .imp
+    (.imp (.not P) (.not Q)) # .imp Q P
+  | mp p₁ p₂ => do match ←p₁.stat, ←p₂.stat with
+    | .imp P Q, P' =>
+      guard # P = P'
+      some Q
+    | _, _ => none
+
+structure Proof (e : Stat) : Prop where
+  h : ∃ (p : Proof'), p.stat = some e
 
 -----
 
-noncomputable
-def Proof.p {e} (h : Proof e) : Proof' e := by
-  apply Nonempty.some; cases h; nm h; use h
+theorem ax₁ (P Q : Stat) : Proof # .imp P # .imp Q P := by
+  use Proof'.ax₁ P Q; rfl
 
-@[match_pattern] def ax₁ P Q := Proof.mk # Proof'.ax₁ P Q
-@[match_pattern] def ax₂ P Q R := Proof.mk # Proof'.ax₂ P Q R
-@[match_pattern] def ax₃ P Q := Proof.mk # Proof'.ax₃ P Q
+theorem ax₂ (P Q R : Stat) : Proof # .imp (.imp P # .imp Q R) # .imp (.imp P Q) # .imp P R := by
+  use Proof'.ax₂ P Q R; rfl
 
-@[match_pattern]
-def mp {P Q : Expr} (h₁ : Proof # .imp P Q) (h₂ : Proof _) :=
-  Proof.mk # Proof'.mp h₁.p h₂.p
+theorem ax₃ (P Q : Stat) : Proof # .imp (.imp (.not P) (.not Q)) # .imp Q P := by
+  use Proof'.ax₃ P Q; rfl
+
+theorem mp {P Q} (h₁ : Proof # .imp P Q) (h₂ : Proof P) : Proof Q := by
+  obtain ⟨p₁, h₁⟩ := h₁; obtain ⟨p₂, h₂⟩ := h₂; use Proof'.mp p₁ p₂; simpa [h₁]
 
 theorem mp' {P Q} (h₁ : Proof P) (h₂ : Proof # .imp P Q) : Proof Q :=
   mp h₂ h₁
 
 theorem imp_refl : Proof # .imp (.var 0) (.var 0) := by
-  generalize Expr.var 0 = P
+  generalize Stat.var 0 = P
   apply mp' # ax₁ P P
   apply mp' # ax₁ P (.imp P P)
   exact ax₂ P (.imp P P) P
 
 @[simp]
-def Expr.subst (e : Expr) (i : ℕ) (e' : Expr) : Expr :=
-  match e with
-  | .var j => if j = i then e' else e
-  | .not e => .not # e.subst i e'
-  | .imp a b => .imp (a.subst i e') (b.subst i e')
+def Stat.subst (s : Stat) (i : ℕ) (s' : Stat) : Stat :=
+  match s with
+  | .var j => if j = i then s' else s
+  | .not e => .not # e.subst i s'
+  | .imp a b => .imp (a.subst i s') (b.subst i s')
 
 @[simp]
-def proof_subst_of' {e e' i} (p : Proof' e) : Proof' # e.subst i e' :=
-  match hp : p with
-  | .ax₁ P Q => by nm h₁; subst h₁; simp at hp ⊢; subst hp; apply Proof'.ax₁
-  | .ax₂ P Q R => by nm h₁; subst h₁; simp at hp ⊢; subst hp; apply Proof'.ax₂
-  | .ax₃ P Q => by nm h₁; subst h₁; simp at hp ⊢; subst hp; apply Proof'.ax₃
-  | .mp p₁ p₂ => by
-    nm a b h₁; subst h₁; simp at hp; subst hp; have p₁' := @proof_subst_of' _ e' i p₁
-    have p₂' := @proof_subst_of' _ e' i p₂; simp at p₁'; exact Proof'.mp p₁' p₂'
-termination_by sizeOf p
-decreasing_by all_goals
-  nm a b p' h₁ h₂; subst h₁; simp at h₂ hp; subst h₂; rw [hp]; simp; try linarith
+def Proof'.subst (p : Proof') (i : ℕ) (s : Stat) : Proof' :=
+  match p with
+  | .ax₁ P Q => .ax₁ (P.subst i s) (Q.subst i s)
+  | .ax₂ P Q R => .ax₂ (P.subst i s) (Q.subst i s) (R.subst i s)
+  | .ax₃ P Q => .ax₃ (P.subst i s) (Q.subst i s)
+  | .mp p₁ p₂ => .mp (p₁.subst i s) (p₂.subst i s)
 
-theorem proof_subst_of {e e' i} (h : Proof e) : Proof # e.subst i e' :=
-  ⟨proof_subst_of' h.p⟩
+theorem Proof'.stat_subst_eq_some_of {s s' i} {p : Proof'}
+(h : p.stat = some s) : (p.subst i s').stat = some (s.subst i s') := by
+  induction p generalizing s
+  any_goals try simp at h; simp [←h]
+  nm p₁ p₂ ih₁ ih₂
+  simp at h ⊢
+  choose s₁ hs₁ s₂ hs₂ h using h
+  specialize ih₁ hs₁
+  specialize ih₂ hs₂
+  simp [ih₁, ih₂]
+  split at h <;> simp at h
+  nm s₁' s₂' P' Q'
+  rcases h with ⟨rfl, rfl⟩
+  simp
+
+theorem Proof.subst_of {s s' i} (h : Proof s) : Proof # s.subst i s' := by
+  obtain ⟨p, h⟩ := h; use p.subst i s', p.stat_subst_eq_some_of h
+
+open Classical in noncomputable
+def Proof'.shortest (p : Proof') : Proof' :=
+  Classical.epsilon # λ p₁ => p₁.stat = p.stat ∧
+  ∀ (p₂ : Proof'), p₂.stat = p.stat → sizeOf p₁ ≤ sizeOf p₂
+
+theorem Proof'.shortest_spec {p : Proof'} : p.shortest.stat = p.stat ∧
+∀ (p' : Proof'), p'.stat = p.stat → sizeOf p.shortest ≤ sizeOf p' := by
+  unfold shortest
+  apply Classical.epsilon_spec (p := λ (p₁ : Proof') => p₁.stat = p.stat ∧
+    ∀ (p₂ : Proof'), p₂.stat = p.stat → sizeOf p₁ ≤ sizeOf p₂)
+  have h₁ : ∃ (n : ℕ) (p' : Proof'), p'.stat = p.stat ∧ sizeOf p' = n
+  · simp
+  replace h₁ := Nat.exi_least_of_exi h₁
+  obtain ⟨n, ⟨p', h₁, rfl⟩, h₂⟩ := h₁
+  use p', h₁
+  intro p₂ h₃
+  simp at h₂
+  by_contra! h₄
+  exact h₂ _ h₄ _ h₃ rfl
 
 @[simp]
-def Proof'.nodes {e} (p : Proof' e) : Set # Σ e, Proof' e :=
-  match h₁ : p with
-  | .ax₁ _ _ => {⟨e, p⟩}
-  | .ax₂ _ _ _ => {⟨e, p⟩}
-  | .ax₃ _ _ => {⟨e, p⟩}
-  | .mp p₁ p₂ => by nm e p₃ h₂; subst h₂; exact insert ⟨e, p⟩ # p₁.nodes ∪ p₂.nodes
-termination_by sizeOf p
-decreasing_by all_goals
-  nm a b p' h₂; subst h₂; simp at h₁ hp; subst hp; rw [h₁]; simp; try linarith
+theorem Proof'.stat_shortest {p : Proof'} : p.shortest.stat = p.stat :=
+  shortest_spec.1
 
-@[simp]
-theorem mem_nodes_self {e} {p : Proof' e} : ⟨e, p⟩ ∈ p.nodes := by
-  cases p <;> simp
+theorem Proof.exi_shortest {s} {h : Proof s} : ∃ (p₁ : Proof'), p₁.stat = some s ∧
+∀ (p₂ : Proof'), p₂.stat = some s → sizeOf p₁ ≤ sizeOf p₂ := by
+  obtain ⟨p, h⟩ := h
+  use p.shortest
+  rw [←h]
+  exact Proof'.shortest_spec
 
--- #check 0 #exit
-
-theorem sizeOf_lt_of_mem_nodes {e e'} {p : Proof' e} {p' : Proof' e'}
-(h₁ : ⟨e', p'⟩ ∈ p.nodes) (h₂ : e' ≠ e ∨ ¬(p' ≍ p)) : sizeOf p' < sizeOf p := by
-  fun_induction Proof'.nodes
-  any_goals
-    simp at h₁; rcases h₁ with ⟨rfl, h₁⟩; simp at h₁ h₂; contradiction
-  nm b a p₁ p₂ ih₁ ih₂ h₁; simp
-  rcases h₁ with h₁ | h₁
-  · by_cases h₃ : e' = .imp a b ∧ p' ≍ p₁
-    · rcases h₃ with ⟨rfl, h₃⟩
-      simp at h₃
-      subst h₃
-      linarith
-    rw [not_and_iff_or] at h₃
-    specialize ih₁ p₁ (by simp) h₁ h₃
-    linarith
-  · by_cases h₃ : e' = a ∧ p' ≍ p₂
-    · rcases h₃ with ⟨rfl, h₃⟩
-      simp at h₃
-      subst h₃
-      linarith
-    rw [not_and_iff_or] at h₃
-    specialize ih₂ p₁ (by simp) h₁ h₃
-    linarith
-
-theorem sizeOf_le_of_mem_nodes {e e'} {p : Proof' e} {p' : Proof' e'}
-(h : ⟨e', p'⟩ ∈ p.nodes) : sizeOf p' ≤ sizeOf p := by
-  by_cases h₁ : e' ≠ e ∨ ¬(p' ≍ p)
-  · exact le_of_lt # sizeOf_lt_of_mem_nodes h h₁
-  push_neg at h₁
-  rcases h₁ with ⟨rfl, h₁⟩
-  simp at h₁
-  rw [h₁]
-
--- theorem mem_nodes_of_imp_var {a i} (p₁ : Proof' a) (p₂ : Proof' # .imp a # .var i) :
--- ∃ (p : Proof' # .var i), ⟨_, p⟩ ∈ p₂.nodes := by
---   cases h₁ : p₂
---   nm b p₃ p₄
---   subst h₁
---   simp
---   sorry
--- 
--- -- #check 0 #exit
--- 
 -- @[simp]
--- theorem not_proof_var {i} : ¬Proof (.var i) := by
---   classical
---   rintro h
---   replace h : ∃ (n : ℕ) (p : Proof' # .var i), sizeOf p = n
---   · simp; exact ⟨h.p⟩
---   replace h : ∃ (p : Proof' # .var i), ∀ (p' : Proof' # .var i), sizeOf p ≤ sizeOf p'
---   · replace h := Nat.exi_least_of_exi h
---     rcases h with ⟨n, ⟨p, rfl⟩, h⟩
---     use p
---     intro p'
---     by_contra! h₁
---     specialize h _ h₁
---     simp at h
---   obtain ⟨p, h⟩ := h
---   cases h₁ : p
---   nm b p₁ p₂
---   subst h₁
---   choose p h₁ using mem_nodes_of_imp_var p₁ p₂
---   replace h₁ := sizeOf_lt_of_mem_nodes h₁ (by simp)
---   specialize h p
---   simp at h
---   linarith
+-- theorem Proof.not_var {i} : ¬Proof (.var i) := by
+--   intro h
+--   replace h := h.exi_shortest
+--   obtain ⟨p, h₁, h₂⟩ := h
+--   sorry
